ast: Add an order on names

src/AST/Names.dfy
@@ -1,4 +1,12 @@
+include "../Utils/Library.dfy"
+
 module {:options "-functionSyntax:4"} Bootstrap.AST.Names {
+  import Utils.Lib.Set
+  import C = Utils.Lib.Sort.Comparison
+  import SeqCmp = Utils.Lib.Seq.Comparison
+  import StrCmp = Utils.Lib.Str.Comparison
+  import DerivedCmp = Utils.Lib.Sort.DerivedComparison
+
   type Atom =
     // An individual component of a Dafny name.
     s: string | s != "" && '.' !in s witness "n"
@@ -18,6 +26,36 @@ module {:options "-functionSyntax:4"} Bootstrap.AST.Names {
         case Anonymous => "_"
         case Name(Anonymous, suffix) => suffix
         case Name(parent, suffix) => parent.ToString() + "." + suffix
+    }
+
+    function ToSeq(): seq<Atom> {
+      match this
+        case Anonymous => []
+        case Name(parent, suffix) => parent.ToSeq() + [suffix]
+    }
+
+    static lemma {:induction false} ToSeqInj1(n0: Name, n1: Name)
+      requires n0.ToSeq() == n1.ToSeq()
+      decreases n0.Length()
+      ensures n0 == n1
+    {
+      var s0, s1 := n0.ToSeq(), n1.ToSeq();
+      if s0 != [] && s1 != [] {
+        assert s0 == s0[..|s0| - 1] + [s0[|s0| - 1]];
+        assert s1 == s1[..|s1| - 1] + [s1[|s1| - 1]];
+        assert n0.Name? && n1.Name?;
+        assert n1.suffix == s1[|s1| - 1] == s0[|s0| - 1] == n0.suffix;
+        assert n0.parent.ToSeq() == s0[..|s0| - 1] == s1[..|s1| - 1] == n1.parent.ToSeq();
+        ToSeqInj1(n0.parent, n1.parent);
+      }
+    }
+
+    static lemma ToSeqInj()
+      ensures forall n0: Name, n1: Name | n0.ToSeq() == n1.ToSeq() :: n0 == n1
+    {
+      forall n0: Name, n1: Name | n0.ToSeq() == n1.ToSeq() {
+        ToSeqInj1(n0, n1);
+      }
     }
 
     predicate ChildOf(parent: Name)
@@ -60,6 +98,20 @@ module {:options "-functionSyntax:4"} Bootstrap.AST.Names {
       ensures n2.StrictSuffixOf(n0)
     {
       SuffixOf_Transitive(n0, n1, n2);
+    }
+
+    static const toSeq: Name -> seq<string> := (name: Name) => name.ToSeq();
+    static const AtomSeqComparison := SeqCmp.SeqComparison(StrCmp.Comparison);
+    static const NameComparison := DerivedCmp.DerivedComparison(AtomSeqComparison.Comparison, toSeq);
+    static const Comparison := NameComparison.Comparison;
+
+    static lemma {:induction false} Total(names: set<Name>)
+      ensures Comparison.Total?(names)
+    {
+      ToSeqInj();
+      StrCmp.Total(SeqCmp.Flatten(Set.Map(names, toSeq)));
+      AtomSeqComparison.Total(Set.Map(names, toSeq));
+      NameComparison.Total(names);
     }
   }
 }
